src/DCE.v
@@ -1,61 +1,56 @@
-Require Import Common FirstOrder. 
+Require Import Common DList FirstOrder. 
 Require BDD. 
+
+(**  We start by defining a poor man's operations on set of natural numbers *)
+Section attic. 
+  Fixpoint mem n l := 
+    match l with 
+      | nil => false 
+      | cons t q => NPeano.Nat.eqb n t || mem n q 
+    end%bool.
+  
+
+  Fixpoint union (i j: list nat) : list nat :=
+    match i with 
+      | nil => j
+      | t :: q => if mem t j then union q j else union q (t :: j)
+    end%list. 
+End attic. 
 
 Section t. 
   Variable Phi: Core.state.  
   
+  (** Recall that in [FirstOrder] syntax, a Var is just a pair of a [type] and a [nat] *)
   Definition Var_eqb {t} (x: Var t) t'  (y: Var t') : bool :=
     (Core.type_eqb t t' && let (x) := x in let (y) := y in (NPeano.Nat.eqb x y))%bool. 
 
   Notation "x ?= y" := (Var_eqb x _ y) (at level 30). 
-  Section e. 
-    Variable (X: Type) (F: X -> Type).
-    Variable (f: forall (x: X) (dx: F x), bool). 
-    Fixpoint existb (l: list X) (dl: DList.T F l) : bool :=
-      match dl with 
-        | DList.nil => false
-        | DList.cons t q dt dq => (f t dt || existb q dq)%bool
-      end.
-  End e. 
-  Arguments existb {X F} _ {l} dl%dlist. 
-
+  
+  (** We define what it means for an expression to use a given variable *)
   Definition use {t t'} (n:Var t) (x: RTL.expr Phi Var t') : bool :=
     match x with
       | RTL.Evar t' m => n ?= m
       | RTL.Eread t x => false
       | RTL.Eread_rf n t x x0 => false
-      | RTL.Ebuiltin tys res f args => existb (Var_eqb n) args
+      | RTL.Ebuiltin tys res f args => DList.existb (Var_eqb n) args
       | RTL.Econstant ty x => false
       | RTL.Emux t c l r => n ?= c || n ?= l || n ?= r
       | RTL.Efst l t x => n ?= x 
       | RTL.Esnd l t x => n ?= x
       | RTL.Enth l t v x => n ?= x
-      | RTL.Etuple tys args => existb (Var_eqb n) args
+      | RTL.Etuple tys args => DList.existb (Var_eqb n) args
     end%bool.
 
   Notation Gamma := (list ({t: Core.type & RTL.expr Phi Var t})). 
   
-  Section foldo.
-    Variable X : Type. Variable F G: X -> Type. 
-    Variable f: forall (x:X) (dx: F x), option (G x). 
-    
-    Fixpoint mapo (l:list X) (dl: DList.T F l) : option (DList.T G l) :=
-      match dl with 
-        | DList.nil => Some (DList.nil)
-        | DList.cons t q dt dq => 
-            do dt <- f t dt;
-            do dq <- mapo q dq;
-            Some (dt :: dq)
-      end%dlist. 
-  End foldo. 
-  Arguments mapo {X F G} _ {l} dl%dlist. 
-
+  (** [get map x] tries to associate the index of [x] in the substitution [map]*)
   Definition get {t} map (x: Var t) := 
     let (x) := x in
-      do x <- BDD.assoc NPeano.Nat.eqb x map; Some  (box t x). 
+      (do x <- BDD.assoc NPeano.Nat.eqb x map; 
+       Some  (box t x)). 
 
-
-  Definition update_expr (map: list (nat * nat)) {t} (e: RTL.expr Phi Var t) :
+  (** [subst_expr map e] applies the subsitution [map] to the expression [e] *)
+  Definition subst_expr (map: list (nat * nat)) {t} (e: RTL.expr Phi Var t) :
     option (RTL.expr Phi Var t) :=
     let get {t} x := get map x in 
     match e in RTL.expr _ _ t return option (RTL.expr Phi Var t)with
@@ -67,7 +62,7 @@ Section t.
           do adr <- get adr;
           Some (RTL.Eread_rf v adr)
       | RTL.Ebuiltin tys res f args => 
-          do args <- mapo (@get) args;
+          do args <- DList.mapo (@get) args;
           Some (RTL.Ebuiltin f args)          
       | RTL.Econstant ty x => Some (RTL.Econstant x)
       | RTL.Emux t c l r => 
@@ -83,32 +78,31 @@ Section t.
           do x <- get x;
           Some (RTL.Enth v x)
       | RTL.Etuple tys args =>
-          do args <- mapo (@get) args;
+          do args <- DList.mapo (@get) args;
           Some (RTL.Etuple args)          
     end%bool.
   
+  (** [ise_used n G] tests whether the variable [n] is used in the bindings [G]  *)
   Fixpoint is_used {t} (n: Var t) (G: Gamma) : bool :=
     match G with 
       | nil => false
       | cons (existT  _ e) q => use n e || is_used (n) q 
     end%bool. 
 
+  (** [crop preserve _ _ map G] sift through the bindings [G] to remove
+  the unused ones, and accumulates a substitution [map] that is used
+  to update the bindings that are kept.  *)
+
   Section crop. 
     Variable preserve: list nat.
-    Fixpoint mem n l := 
-      match l with 
-        | nil => false 
-        | cons t q => NPeano.Nat.eqb n t || mem n q 
-      end%bool.
-
  
-    Fixpoint crop old next (map: list (nat * nat)) (bindings: Gamma) : option (list (nat * nat) * Gamma) :=
-      match bindings with 
-        | nil => Some (map, nil)
+    Fixpoint crop old next (map: list (nat * nat)) (G: Gamma) : option (list (nat * nat) * Gamma) :=
+      match G with 
+        | nil => Some ((old, next) :: map, nil)
         | cons (existT t e) q => 
             if (mem old preserve) || is_used (box t old) q
             then 
-              do e <- (update_expr map e);
+              do e <- (subst_expr map e);
               do map, q <- crop (S old) (S next) ((old,next) :: map) q;
               Some (map,cons (existT _ t e) q)
             else
@@ -118,28 +112,32 @@ Section t.
 
   Notation Xi := (DList.T (option ∘ RTL.effect Var) Phi). 
 
-  Definition update_effect {t} (map: list (nat * nat)) (e: RTL.effect Var t):
+  Definition subst_effect {t} (map: list (nat * nat)) (e: RTL.effect Var t):
     option (RTL.effect Var t) :=
- (match e  with
-            | RTL.effect_reg_write t value guard =>
-                do value <- get map value;
-                do guard <- get map guard;
-                Some (RTL.effect_reg_write _ (t) value guard)
-            | RTL.effect_regfile_write n t value adr guard =>
-                do value <- get map value;
-                do guard <- get map guard;
-                do adr <- get map adr;
-                Some (RTL.effect_regfile_write _ _ _ value adr guard)
-          end). 
+    (match e  with
+       | RTL.effect_reg_write t value guard =>
+           do value <- get map value;
+           do guard <- get map guard;
+           Some (RTL.effect_reg_write _ (t) value guard)
+       | RTL.effect_regfile_write n t value adr guard =>
+           do value <- get map value;
+           do guard <- get map guard;
+           do adr <- get map adr;
+           Some (RTL.effect_regfile_write _ _ _ value adr guard)
+     end). 
 
-  Definition update_effects (map: list (nat * nat)) (dl: Xi) : option Xi.
-  refine (mapo _ dl).
-  intros. 
-  destruct dx. apply (update_effect map) in e. apply (Some (e)). 
-  refine None.
-  Defined. 
+  (** [subst_effect map dl] applies the substitution [map] on every
+  element of [dl] *)
 
-  
+  Definition subst_effects (map: list (nat * nat)) (dl: Xi) : option Xi :=
+    DList.mapo (fun x dx =>
+                  let t :=  comp option (RTL.effect Var) x in  
+                    match dx : t return option t with
+                    | Some e => do x <- (subst_effect map e); Some (Some x)
+                    | None => Some None
+                  end) dl. 
+
+  (** [used e] gather the set of variables used by the effect [e]   *)
   Definition used {t} (e: RTL.effect Var t) := 
     match e with 
       | RTL.effect_reg_write _ v g => 
@@ -153,28 +151,11 @@ Section t.
           [v; g; a]%list
     end. 
       
-  Section fold.
-    Variable A X : Type. Variable F : X -> Type. 
-    Variable f: forall (x:X) (dx: F x), A -> A. 
-    
-    Fixpoint fold (l:list X) (dl: DList.T F l) acc: A :=
-      match dl with 
-        | DList.nil => acc
-        | DList.cons t q dt dq => 
-            f t dt (fold q dq acc)
-      end%dlist. 
-  End fold. 
+  (** [used_effects x l] gather the set of variables used by the
+  effects in [x], and adds it to the set represented by [l] *)
 
-  Arguments fold {A X F} f {l} dl%dlist acc. 
-
-  Fixpoint union (i j: list nat) : list nat :=
-    match i with 
-      | nil => j
-      | t :: q => if mem t j then union q j else union q (t :: j)
-    end%list. 
-    
   Definition used_effects (x : Xi) l :=
-    fold (fun _ e acc => 
+    DList.fold (fun _ e acc => 
             match e with 
                 None => acc 
               | Some e => union (used e) acc
@@ -189,7 +170,7 @@ Section t.
     do map, bindings <- crop preserve 0 0 nil (bindings _ _ b);
     do guard <- BDD.assoc NPeano.Nat.eqb guard map;
     do value <- BDD.assoc NPeano.Nat.eqb value map;
-    (* do effects <- update_effects map (effects _ _ b); *)
+    do effects <- subst_effects map effects;
     Some (mk Phi t bindings (box _ value) (box _ guard) effects).
 End t. 
   
