src/DList.v
@@ -1,0 +1,320 @@
+
+Require List Common. 
+
+Import Common. 
+
+Open Scope list_scope. 
+
+Notation "[ ]" := nil : list_scope.
+Notation "t :: q" := (cons t q) : list_scope. 
+Notation "[ a ; .. ; b ]" := (a :: .. (b :: []) ..)%list : list_scope.
+
+Module DList. 
+Section t. 
+  
+  Variable X : Type. 
+  Variable P : X -> Type. 
+ 
+  Inductive T  : list X -> Type := 
+  | nil : T nil
+  | cons : forall (t : X) q, P t -> T q -> T (cons t q).  
+  
+  Arguments cons t q%list _ _%dlist. 
+  Arguments T _%list. 
+
+  Definition hd t q (x : T (t::q)): P t :=
+    match x as y in T l return
+       (match l return (T l -> Type) with 
+         | [ ] => fun _ : T [] => ID
+         | a::b => fun _ : T (a :: b) => P a
+        end%list y)
+    with 
+      | nil => @id
+      | cons _ _ t q => t
+    end.
+  
+  Definition tl t q (x : T (t::q)): T q :=
+    match x as y in T l return
+       (match l return (T l -> Type) with 
+         | [] => fun _ : T [] => ID
+         | a::b => fun _ : T (a :: b) => T b
+        end%list y)
+    with 
+      | nil => @id
+      | cons _ _ t q => q
+    end.
+
+
+  Fixpoint get l t (v: var l t): T l -> P t :=
+    match v with 
+      | var_0  _ _ => fun e => hd _ _ e
+      | var_S _ _ _ v => fun e => get _ _ v  (tl _ _ e)
+      end. 
+
+  Fixpoint set l t (v : var l t) : P t ->  T l -> T l:=
+    match v  with 
+        | var_0 _ _ => fun x e => cons _ _  x (tl _ _ e)
+        | var_S _ _ _ v => fun x e => cons _ _  (hd _ _ e) (set _ _ v x (tl _ _ e))
+    end. 
+
+  (** * Operations  *)
+  Fixpoint Forall (Q: forall (x : X), P x -> Prop) l (dl : T l) :=
+    match dl with 
+      | nil => True
+      | cons t q dt dq => Q t dt /\ Forall Q q dq
+    end. 
+  
+  Fixpoint init (el : forall t, P t) l : T l :=
+    match l with 
+      | List.nil => nil
+      | List.cons t q => cons _ _ (el t) (init el q)
+    end. 
+  
+  (** * Concatenation of T (append)  *)
+  Definition app : forall (l1 l2 : list X), 
+                         T l1 -> T l2 -> T (List.app l1 l2).   
+  refine (
+      (fix app (l1 l2 : list X) {struct l1} :
+       T l1 -> T l2 -> T (l1 ++ l2) :=
+       match l1 as l3 return (T l3 -> T l2 -> T (l3 ++ l2)) with
+         | [] => fun (_ : T []) (dl2 : T l2) => dl2
+         | (t :: q)%list =>
+             fun (dl1 : T (t :: q)) (dl2 : T l2) =>
+               cons t (q ++ l2)%list (hd t q dl1)
+                          (app q l2 (tl t q dl1) dl2)
+      end%list)). 
+  Defined. 
+  
+
+  (* (** * Other functions operating on tuples like things *) *)
+  (* Variable E : X -> Type. *)
+  
+  (* Section foldo.  *)
+  (*   Variable F : forall (t : X), P t -> E t -> option (E t).  *)
+  (*   Fixpoint fold (l : list X) (d : T l) : Tuple.of_list E l -> option (Tuple.of_list E l):= *)
+  (*     match d with *)
+  (*         nil => fun v => Some v *)
+  (*       | cons t q pt dlq => fun v => *)
+  (*           do x <- F t pt (fst v); *)
+  (*           do y <- fold q dlq (snd v); *)
+  (*           Some (x,y) *)
+  (*     end. *)
+  (* End foldo.  *)
+
+  (* Section s2.  *)
+
+  (*   Variable F : forall (t : X), P t -> E t.  *)
+
+  (*   Definition fold' (l : list X) (dl : T l) : Tuple.of_list E l.  *)
+  (*   induction dl. simpl. apply tt.  *)
+  (*   simpl. destruct q. auto. split. auto. auto.  *)
+  (*   Defined.  *)
+  (* End s2.  *)
+
+End t. 
+
+Arguments T {X} P _%list. 
+Arguments nil {X P}. 
+Arguments cons {X P} {t q} _ _%dlist.  
+
+Arguments app {X P l1 l2} _%dlist _%dlist. 
+Arguments get {X P l t} _ _%dlist.  
+Arguments set {X P l t} _ _ _%dlist.  
+
+Arguments Forall {X P} _ {l}%list _%dlist. 
+Arguments init {X P} _ l%list.
+
+Section ops. 
+  Variable X : Type. 
+  Variable (F G : X -> Type). 
+  Variable (Op : forall x, F x -> G x). 
+  Definition to_tuple (l : list X) : T F l -> Tuple.of_list G l. 
+  refine ((fix F l (hl : T F l) : Tuple.of_list G l :=
+           match hl in T _ l return Tuple.of_list G l with 
+                                  | nil => tt
+                                  | cons t q T Q =>  ((Op t T),(F q Q))
+           end) l).
+  Defined. 
+
+  Definition to_etuple (l : list X) : T F l -> ETuple.of_list G l. 
+  refine ((fix F l (hl : T F l) : ETuple.of_list G l :=
+           match hl in T _ l return ETuple.of_list G l with 
+                                  | nil => tt
+                                  | cons t q T Q =>  ETuple.pair X G (Op t T) (F q Q)
+           end) l).
+  Defined. 
+  
+  Definition map ( l : list X) : T F l -> T G l. 
+  refine ((fix F l (hl : T F l) : T G l := 
+          match hl in T _ l return T G l with 
+            | nil => nil
+            | cons t q T Q => cons (Op _ T) (F _ Q)
+          end) l). 
+  Defined. 
+End ops. 
+Arguments to_tuple {X F G} Op {_} _%dlist. 
+Arguments to_etuple {X F G} Op {_} _%dlist. 
+Arguments map {X F G} Op {_} _%dlist. 
+
+Lemma map_to_tuple_commute {X} (F G H : X -> Type)
+                            (Op : forall x, F x -> G x) (Op' : forall x : X, G x -> H x)
+                            (l : list X) (dl : T F l) :
+  to_tuple Op' (map Op dl) = 
+  to_tuple (fun x dx => Op' x (Op x dx)) dl. 
+Proof.
+  induction dl. reflexivity.
+  simpl. f_equal. apply IHdl. 
+Qed. 
+
+
+Lemma map_to_etuple_commute {X} (F G H : X -> Type)
+                            (Op : forall x, F x -> G x) (Op' : forall x : X, G x -> H x)
+                            (l : list X) (dl : T F l) :
+  to_etuple Op' (map Op dl) = 
+  to_etuple (fun x dx => Op' x (Op x dx)) dl. 
+Proof.
+  induction dl. reflexivity.
+  simpl. f_equal. apply IHdl. 
+Qed. 
+  
+Definition hmap :
+  forall (X Y : Type) (P : Y -> Type) (Q : X -> Type)
+    (F :  X -> Y), 
+    (forall x : X, P (F x) -> Q x) -> forall l : list X, T P (List.map F l) -> T Q l. 
+induction l. simpl. constructor. 
+simpl. intros. inversion X1.   subst. constructor. auto. auto. 
+Defined. 
+
+Definition dmap {A B} (F : A -> Type) (G: B -> Type) (C : A -> B) (D : forall x, F x -> G ( C x)) (l: list  A) (dl : T F l) : T G (List.map C l). 
+  induction dl. simpl. constructor. 
+  simpl. constructor. apply D.  auto. 
+  apply IHdl. 
+Defined. 
+
+Inductive pointwise {A} F G (R : forall a, F a -> G a -> Prop): forall (l : list A), T F l -> T G l -> Prop :=
+| pointwise_nil : pointwise F G R List.nil nil nil
+| pointwise_cons : forall t q dt1 dt2 dq1 dq2,
+                     R t dt1 dt2 -> 
+                     pointwise F G R q dq1 dq2 ->
+                     pointwise F G R (t::q) (cons dt1 dq1) (cons dt2 dq2). 
+Arguments hd {X P t q} _%dlist.  
+Arguments tl {X P t q} _%dlist.  
+Section map3. 
+  Context {X : Type} {F F' F'': X -> Type}.
+  Variable (up : forall a,  F a -> F' a -> F'' a -> F'' a). 
+  Fixpoint map3 l : T F l -> T F' l -> T F'' l -> T F'' l :=
+    match l with 
+      | List.nil => fun _ _ x => x
+      | List.cons t q => fun xs ys zs => 
+                         let (x,xs) := (hd xs, tl xs) in 
+                         let (y,ys) := (hd ys, tl ys) in 
+                         let (z,zs) := (hd zs, tl zs) in 
+                           cons (up t x y z)  (map3 q xs ys zs)
+    end. 
+End map3. 
+
+Section map3o. 
+  Context {X : Type} {F F' F'': X -> Type}.
+  Variable (up : forall a,  F a -> F' a -> F'' a -> option (F'' a)). 
+  Fixpoint map3o l :  T F l ->  T F' l ->  T F'' l -> option (T F'' l) :=
+    match l with 
+        | List.nil => fun _ _ x => Some x
+        | List.cons t q => fun xs ys zs => 
+                         let (x,xs) := (hd xs, tl xs) in 
+                         let (y,ys) := (hd ys, tl ys) in 
+                         let (z,zs) := (hd zs, tl zs) in 
+                           do t <- up t x y z;
+                           do q <- map3o q xs ys zs;
+                           Some (cons t q) 
+    end. 
+End map3o. 
+
+Require Import Equality.
+
+Lemma inversion_dlist_cons {A F} : forall (t : A) q (dl : T F (t :: q)), 
+                              exists hd tl, dl = (cons hd tl)%dlist. 
+Proof. 
+  intros.  dependent destruction dl. eauto. 
+Qed. 
+
+Lemma inversion_dlist_nil {A} {F : A -> Type}  (dl : T F []) :
+                              dl = (nil)%dlist. 
+Proof. 
+  dependent destruction dl. reflexivity. 
+Qed. 
+
+Require Import Equality.
+Lemma inversion_pointwise {A F G} P (t : A) q dt dq dt' dq':
+  pointwise F G P (t :: q)%list (cons dt dq) (cons dt'  dq') ->
+  pointwise F G P q dq dq' /\ P t dt dt'. 
+Proof. 
+  intros H.  
+  inversion H;
+    repeat match goal with 
+               H : existT _ _ _ = existT _ _ _ |- _ => apply Eqdep.EqdepTheory.inj_pair2 in H
+           end; subst; auto. 
+Qed. 
+
+Ltac inversion :=
+  match goal with 
+    | H : DList.T _ (_ :: _) |- _ => 
+        destruct (inversion_dlist_cons _ _ H) as [? [? ?]]
+    | H : DList.T _ ([]) |- _ => 
+        pose proof (inversion_dlist_nil H)
+  end; subst. 
+
+Arguments DList.pointwise {A F G} _ l%list _%dlist _%dlist. 
+
+(** * [existb f dl] tests whether an element of [dl] satisfies the predicate [f] *)
+Section existb. 
+  Variable (X: Type) (F: X -> Type).
+  Variable (f: forall (x: X) (dx: F x), bool). 
+  Fixpoint existb (l: list X) (dl: T F l) : bool :=
+    match dl with 
+      | DList.nil => false
+      | DList.cons t q dt dq => (f t dt || existb q dq)%bool
+    end.
+End existb. 
+Arguments existb {X F} _ {l} dl%dlist. 
+
+(** [mapo f dl] applies the partial function [f] to every element of
+[dl]. If any such application fails (i.e., returns [None]), then [mapo
+f dl] fails.  *)
+
+Section mapo.
+  Variable (X : Type). Variable F G: X -> Type. 
+  Variable f: forall (x:X) (dx: F x), option (G x). 
+  
+  Fixpoint mapo (l:list X) (dl: DList.T F l) : option (DList.T G l) :=
+    match dl with 
+      | DList.nil => Some (DList.nil)
+      | DList.cons t q dt dq => 
+          do dt <- f t dt;
+          do dq <- mapo q dq;
+          Some (cons dt dq)
+    end%dlist. 
+End mapo. 
+Arguments mapo {X F G} _ {l} dl%dlist. 
+
+(** [fold f dl acc] fold the function [f] through [dl], starting with
+the accumulator [acc]. The type of the accumulator is static. *)
+
+Section fold.
+  Variable X A: Type. Variable F : X -> Type. 
+  Variable f: forall (x:X) (dx: F x), A -> A. 
+  
+  Fixpoint fold (l:list X) (dl: DList.T F l) acc: A :=
+    match dl with 
+      | DList.nil => acc
+      | DList.cons t q dt dq => 
+          f t dt (fold q dq acc)
+    end%dlist. 
+End fold. 
+
+Arguments fold {X A F} f {l} dl%dlist acc. 
+
+End DList. 
+
+Notation "[ :: ]" := DList.nil : dlist_scope.
+Notation "t :: q" := (DList.cons t q) : dlist_scope.
+Notation "[ :: a ; .. ; b ]" := (a :: .. (b :: [ :: ]) ..)%dlist : dlist_scope.
